\documentclass[12pt]{article}

\usepackage{prooftrees,amsmath,turnstile,amsthm}
\usepackage{tikz}
\usepackage{tikz-qtree}

\usepackage{graphicx}
\graphicspath{ {./imgs/} }

\title{Symbolic Logic HW 3}
\author{Tyler Tracy}

\newtheorem{theorem}{Theorem}

\begin{document}

\maketitle

\section*{Solution to Problem 1}

\[\exists x(Fx \land \neg Gx) \leftrightarrow (\forall x Fx \rightarrow \forall xGx)\]

\begin{figure}[h]
\centering
\begin{tikzpicture}
\tikzset{grow=down,level distance=32pt}
\Tree
[.\(\leftrightarrow\)
    [ .\(\exists x\)
        [ .\(\land\)
            [ .\(Fx\) ]
            [ .\(\neg Gx\) ]
        ]
    ]
    [.\(\rightarrow\)
        [.\(\forall x\)
            [.\(Fx\) ]
        ]
        [.\(\forall x\)
            [.\(Gx\) ]
        ]
    ]
]
\end{tikzpicture}
\end{figure}

The main logical operator is $\leftrightarrow$. 
The $\exists x$ in $\exists x (Fx \land \neg Gx)$ has scope over $Fx \land \neg Gx$

The $\forall x$ in $\forall x Fx$ has scope over $Fx$ and $\forall x Gx$ has scope over $Gx$.
The $\rightarrow$ in $\forall x Fx \rightarrow \forall xGx$ has scope over $\forall x Fx$ and $\forall xGx$.


\[ \forall x (Ax \leftrightarrow Bx) \rightarrow \exists (Ax \land Bx) \]

\begin{center}
\begin{tikzpicture}
\tikzset{grow=down,level distance=32pt}
\Tree
[.\(\rightarrow\)
    [ .\(\forall x\)
        [ .\(\leftrightarrow\)
            [ .\(Ax\) ]
            [ .\(\neg Bx\) ]
        ]
    ]
    [.\(\exists\)
        [.\(\land x\)
            [.\(Ax\) ]
            [.\(Bx\) ]
        ]
    ]
]
\end{tikzpicture}
\end{center}


The main logical operator is $\rightarrow$. It's scope is over $\forall x (Ax \leftrightarrow Bx)$ and $\exists (Ax \land Bx)$.
The $\forall x$ in $\forall x (Ax \leftrightarrow Bx)$ has scope over $Ax \leftrightarrow Bx$.
The $\exists x$ in $\exists (Ax \land Bx)$ has scope over $Ax \land Bx$.
The $\leftrightarrow$ in $Ax \leftrightarrow Bx$ has scope over $Ax$ and $Bx$.
The $\land$ in $Ax \land Bx$ has scope over $Ax$ and $Bx$.


\[ (\forall x Fx \rightarrow \forall x Gx) \rightarrow \forall x (Fx \rightarrow Gx) \]

\begin{center}
\begin{tikzpicture}
\tikzset{grow=down,level distance=32pt}
\Tree
[.\(\rightarrow\)
    [ .\(\forall x\)
        [ .\(\rightarrow\)
            [ .\(\forall x\)
                [ .\(Fx\) ]
            ]
            [ .\(\forall x\)
                [ .\(Gx\) ]
            ]
        ]
    ]
    [.\(\forall x\)
        [.\(\rightarrow\)
            [.\(Fx\) ]
            [.\(Gx\) ]
        ]
    ]
]
\end{tikzpicture}
\end{center}

The main logical operator is $\rightarrow$. It's scope is over $(\forall x Fx \rightarrow \forall x G)$ and $\forall x (Fx \rightarrow Gx)$.
The $\forall x$ in $\forall x Fx$ has scope over $Fx$.
The $\forall x$ in $\forall x Gx$ has scope over $Gx$.
The $\rightarrow$ in $\forall x Fx \rightarrow \forall x Gx$ has scope over $\forall x Fx$ and $\forall x Gx$.
The $\forall x$ in $\forall x (Fx \rightarrow Gx)$ has scope over $Fx \rightarrow Gx$.
The $\rightarrow$ in $Fx \rightarrow Gx$ has scope over $Fx$ and $Gx$.




\[ \forall x (Ax \rightarrow Bx) \lor \forall x( \neg Ax \rightarrow Bx) \]

\begin{center}
\begin{tikzpicture}
\tikzset{grow=down,level distance=32pt}
\Tree
[.\(\lor\)
    [ .\(\forall x\)
        [ .\(\rightarrow\)
            [ .\(Ax\) ]
            [ .\(Bx\) ]
        ]
    ]
    [.\(\forall x\)
        [.\(\rightarrow\)
            [.\(\lnot Ax\) ]
            [.\(Bx\) ]
        ]
    ]
]

\end{tikzpicture}
\end{center}

The main logical operator is $\lor$. It's scope is over $\forall x (Ax \rightarrow Bx)$ and $\forall x( \neg Ax \rightarrow Bx)$.
The $\forall x$ in $\forall x (Ax \rightarrow Bx)$ has scope over $Ax \rightarrow Bx$.
The $\forall x$ in $\forall x( \neg Ax \rightarrow Bx)$ has scope over $\neg Ax \rightarrow Bx$.
The $\rightarrow$ in $Ax \rightarrow Bx$ has scope over $Ax$ and $Bx$.
The $\rightarrow$ in $\neg Ax \rightarrow Bx$ has scope over $\neg Ax$ and $Bx$.
The $\neg$ in $\neg Ax$ has scope over $Ax$.


\section*{Solution to Problem 2}

Convert the following predicate logic sentences into English.

\[ \exists x (Fx \land \neg Gx) \]

There is a fish that doesn't have gills.

\[ \neg \exists x (Fx \land \neg Gx) \]

There is not a fish that doesn't have gills.

\[ \forall x Fx \rightarrow \forall x Gx \]

If everything is a fish, then everything has gills.

\[ \forall x (Fx \rightarrow Gx) \]

All fish have gills.

\[ \forall x ((Fx \land Tx) \rightarrow Gx) \]

Every fish with a tail has gills.

\[ \forall x ((Fx \lor Tx) \rightarrow Gx) \]

Every fish or tailed creature has gills.

\[ \forall x (Fx \lor \neq Fx) \]

Everything is either a fish or not a fish.

\[ \forall x Fx \lor \forall x \neg Fx \]

Either everything is a fish or nothing is a fish.


\section*{Solution to Problem 3}

Translate the following sentence from English into predicate logic. 

Some metals conduct electricity.
\[ \exists x (Mx \land Cx) \]

No metal conducts electricity.
\[ \neg \exists x (Mx \land Cx) \]

If some metal s don't conduct electricity, then it's not the case that all metals do conduct electricity

\[ (\exists x (Mx \land \neg Cx)) \rightarrow \neg (\forall x (Mx \land Cx)) \]

All hard metals conduct electricity.

\[ \forall x ((Hx \land Mx) \rightarrow Cx) \]

All metals and plastics conduct electricity.

\[ \forall x ((Mx \lor Px) \rightarrow Cx) \]

Rhinos exist, but unicorns do not.

\[ \exists x Rx \land \neg \exists x Ux \]

\section*{Solution to Problem 5}

State the truth-values of the listed

sentences on the following interpretation:

Domain = {1, 2, 3, 4, 5}


$F \rightarrow \{1, 2\}$

$G \rightarrow \{1, 2, 3, 4\}$

$L \rightarrow \{<1,1>, <1,2>, <1,3>, <1, 5>, <2, 2>, <3, 1>, <3,2>,<4, 2>, <5, 2>\}$

$a \rightarrow 2$

\[ \forall x Gx \]
False, 5 is not in G.

\[ \forall x(Fx \rightarrow Gx) \]
True, all elements of F are in G.

\[ \exists x(Gx \land \lnot Fx) \]
True, Every element is either in G or not in F.

\[ \forall x F x \rightarrow \forall x G x \]
True, the condition is false. 

\[ \forall x Lxa \]
True, L maps every value in x to the value 2

\[ \forall x Lax \]
False, L doesn't map 2 to every value in x

\[ \forall x Lxx \]
False, L doesn't map 3 to itself

\[ \forall x(Fa \rightarrow Lax) \]
False, L doesn't map 2 to every value in x


\section*{Solution to Problem 6}

\subsection*{Problem a}
\includegraphics[width=\textwidth]{6a}

\subsection*{Problem b}
\includegraphics[width=\textwidth]{6b}

\subsection*{Problem c}
\includegraphics[width=\textwidth]{6c}

\subsection*{Problem d}
\includegraphics[width=\textwidth]{6d}

\section*{Solution to Problem 7}

Prove rule-soundness of the tree rules for the conditional and the negated conditional.

Rule Soundness: if the premise/input is true in some case/valuation C, then all the lines in at least one of its conclusions/outputs is true in case C too.

\begin{theorem}[Conditional Rule Soundness]
    If $A \rightarrow B$ is true in some case/valuation C, then all the lines in one the tree rule's outputs must be true
\end{theorem}

\begin{proof}
    The conditional tree rule is as follows: $A \rightarrow B$ creates a single line with two branches $A$ and $\neg B$. 
    \begin{itemize}
        \item Assume $A \rightarrow B$ is true in some case/valuation C.
        \item $A \rightarrow B$ has the same truth table as $\neg A \lor B$.
        \item In C, either $A$ is false or $B$ is true.
        \item The $A$ branch is true in C when the value of $A$ is true in C.
        \item The $\neg B$ branch is true in C when the value of $B$ is false in C.
        \item That is all the possible cases or C. So if C is true, then one of the branches are true. 
    \end{itemize}
\end{proof}


\section*{Solution to Problem 8}
 Prove the rule-completeness of the tree rules for the biconditional and the negated biconditional.  
 
Rule Completeness:  If all the lines in one of its conclusions/outputs  is true in some case/valuation C, the premise/input is true in C also.


\begin{theorem}[Biconditional Rule Completeness]
    If $A \leftrightarrow B$ is true in some case/valuation C, then $A \rightarrow B$ and $B \rightarrow A$ are true in C also.
\end{theorem}

\begin{proof}

    The biconditional tree rule is as follows:
    $A \leftrightarrow B$ creates a single line with two branches:
    \begin{itemize}
        \item $A \rightarrow B$
        \item $B \rightarrow A$
    \end{itemize}

    We show that

    \begin{itemize}
        \item Assume $A \leftrightarrow B$ is true in some case/valuation C. 
        \item $A \leftrightarrow B$ has the same truth table as $(A \rightarrow B) \land (B \rightarrow A)$.
    \end{itemize}

    By defintion of biconditional, $A \leftrightarrow B$ is true in C if and only if $A$ and $B$ have the same truth value in C.
    Then $A \rightarrow B$ and $B \rightarrow A$ are true in C.
    Therefore, if $A \leftrightarrow B$ is true in some case/valuation C, then $A \rightarrow B$ and $B \rightarrow A$ are true in C also.

\end{proof}



\section*{Solution to Problem 9}



\end{document}

